src/coq/TopLevelRefinements.v
@@ -76,3 +76,80 @@ Proof.
     eapply subrelation_prod_left. apply subrelation_R_TT. apply PR.
   - apply eutt_interp_state_gen; auto.
 Qed.
+
+Instance refine_uvalue_refl :
+  Reflexive refine_uvalue.
+Proof.
+  unfold Reflexive. intros x.
+  induction x; constructor; auto.
+Qed.
+
+Instance TT_refl :
+  forall A, Reflexive (@TT A).
+Proof.
+  firstorder.
+Qed.
+
+Lemma model_refines :
+  forall t1 t, (model_L4 t1) t -> refine_L4 (fun t' => t = t') (model_L4 t1).
+Proof.
+  intros t1 t H.
+  unfold refine_L4. intros t' Heq.
+  exists t. split; auto.
+  subst.
+
+  apply Reflexive_eqit.
+  repeat apply prod_rel_refl; auto using TT_refl, refine_uvalue_refl.
+Qed.
+
+Instance interp_prop_Proper :
+  forall R E F G (t : itree (E +' G) R) (RR : relation R) (h : (E +' F +' G) ~> PropT.PropT (itree (E +' G))),
+    Proper (@eutt (E +' F +' G) _ _ RR ==> iff) (fun t' => @PropT.interp_prop (E +' F +' G) _ _ _ _ h _ t' t).
+Proof.
+  intros R E F G t RR h.
+  intros t1 t2 Heutt.
+  unfold PropT.PropT in h. unfold Ensembles.Ensemble in h.
+Admitted.
+
+Lemma refine_34 : forall t1 t2,
+    refine_L3 t1 t2 -> refine_L4 (model_L4 t1) (model_L4 t2).
+Proof.
+  intros t1 t2 H.
+  unfold refine_L4.
+  intros t Hip.
+
+  unfold model_L4 in *.
+  unfold P.model_undef in *.
+
+  exists t; split.
+
+  match goal with
+  | [ |- context [PropT.interp_prop ?h _ _] ] =>
+    apply (interp_prop_Proper res_L3 _ _ _ t refine_res3 h t1 t2 H)
+  end.
+
+  apply Hip.
+
+  apply Reflexive_eqit.
+  repeat apply prod_rel_refl; auto using TT_refl, refine_uvalue_refl.
+Qed.
+
+
+(* Unfinished proof *)
+(*
+Lemma refine_34_concrete : forall t1 t2,
+    refine_L3 t1 t2 -> refine_L4_concrete (build_L4 t1) (build_L4 t2).
+Proof.
+  intros t1 t2 H.
+  unfold refine_L4_concrete.
+  unfold refine_L3 in H.
+
+  eapply eqit_mon.
+  apply id. apply id.
+
+  intros x0 x1 PR.
+  unfold refine_res4.
+  eapply subrelation_prod_left. apply subrelation_R_TT with (R:=eq). apply PR.
+  
+Qed.
+*)
